LogicalRefinement/Stlc/Utils.lean
@@ -1,0 +1,33 @@
+import LogicalRefinement.Untyped
+import LogicalRefinement.Typed
+import LogicalRefinement.Stlc.Basic
+import LogicalRefinement.Stlc.Interp
+import LogicalRefinement.Stlc.InterpInv
+import LogicalRefinement.Stlc.InterpSubst
+import LogicalRefinement.Stlc.InterpWk
+import LogicalRefinement.Stlc.Subst
+
+open Annot
+
+set_option pp.explicit true
+
+theorem HasVar.stlc_var {Γ n A} (H: HasVar Γ n (HypKind.val type) A)
+  : (Term.var n).stlc Γ.sparsity = Stlc.var (Γ.sparsity.ix n)
+  := by {
+    dsimp only [Term.stlc, Sparsity.stlc]
+    rw [if_pos]
+    rw [H.sigma]
+    sorry
+  }
+
+theorem HasType.stlc_var_term {Γ n A} (H: Γ ⊢ Term.var n: term A)
+  : (Term.var n).stlc Γ.sparsity = Stlc.var (Γ.sparsity.ix n)
+  := by {
+    sorry
+  }
+
+theorem HasType.stlc_interp_var {Γ n A} (H: Γ ⊢ Term.var n: term A):
+  H.stlc.interp = H.to_var.stlc.interp
+  := by {
+    sorry
+  }
